theories/Pipeline.v
@@ -1,0 +1,45 @@
+From MetaCoq.Erasure Require Import ExAst.
+From MetaCoq.Erasure.Typed Require Import Annotations TypeAnnotations Utils.
+From MetaCoq.ErasurePlugin Require Import Erasure Loader.
+From MetaCoq.PCUIC Require Import PCUICAst.
+From MetaCoq.Template Require Import Loader TemplateMonad.
+From MetaCoq.TemplatePCUIC Require Import TemplateToPCUIC.
+From MetaCoq.SafeChecker Require Import PCUICWfEnvImpl.
+From MetaCoq.Utils Require Import utils.
+Import config.
+
+From VTL Require Import PIR Translation.
+
+From Coq.Strings Require Import String.
+Import MCMonadNotation ListNotations.
+
+Local Existing Instance extraction_checker_flags.
+
+Definition gal_id := fun x : nat => x.
+
+Definition plus_one n : nat := n + 1.
+
+(* empty_ext empty_global_env *)
+MetaCoq Quote Recursively Definition gid := 3.
+Eval cbv in run_erase_program typed_erasure_config  gid.
+
+Definition template_to_lt (t : Ast.term) : TemplateMonad (∑ et : EAst.term, annots box_type et) :=
+  match t with
+  | Ast.tConst _ _ => ret (existT (annots box_type) identity_EAst (TArr (TConst <%% bool %%>) (TConst <%% bool %%>), (TConst <%% bool %%>)))
+  | _ => ret (existT (annots box_type) identity_EAst ann_id)
+  end.
+
+Definition compile_pir (t : Ast.term) : TemplateMonad PIR.term :=
+  p <- template_to_lt t ;;
+  match p with | existT et ann =>
+    match translate_term remap_env [] et ann with
+    | Some t' => ret t'
+    | _ => ret (PIR.Error (PIR.UNDEFINED "Not Implemented"))
+    end
+  end.
+
+(* MetaCoq Run ((tmQuoteRec 3) >>= tmEval cbv >>= tmPrint).
+MetaCoq Quote Recursively Definition gid := gal_id.
+Eval cbv in (gid.2). *)
+
+MetaCoq Run (tmQuote gal_id >>= compile_pir >>= tmEval cbn >>= tmPrint).
